RGA set - wip

inductive_proof/RGA_set_pre-cond/App_do_pre_first.fst
@@ -105,8 +105,8 @@ let resolve_conflict_prop (x:op_t) (y:op_t{fst x <> fst y})
 
 // concrete merge pre-condition
 let merge_pre l a b =
-  S.subset (fst l) (fst a) /\ S.subset (fst l) (fst b) /\
-  S.subset (snd l) (snd a) /\ S.subset (snd l) (snd b) /\
+  (*S.subset (fst l) (fst a) /\ S.subset (fst l) (fst b) /\
+  S.subset (snd l) (snd a) /\ S.subset (snd l) (snd b) /\*)
   (forall id. mem_id_s id (fst l) ==> ~ (mem_id_s id (S.difference (fst a) (fst l)))) /\
   (forall id. mem_id_s id (fst l) ==> ~ (mem_id_s id (S.difference (fst b) (fst l)))) /\
   (forall id. mem_id_s id (S.difference (fst a) (fst l)) ==> ~ (mem_id_s id (S.difference (fst b) (fst l))))
@@ -127,13 +127,39 @@ let linearizable_s1_0' (lca s1 s2:st)
   : Lemma (requires consistent_branches lca s1 s2 /\
                     ops_of s1 = ops_of lca /\
                     merge_pre (v_of lca) (v_of s1) (v_of s2))
-          (ensures eq (v_of s2) (concrete_merge (v_of lca) (v_of s1) (v_of s2))) = ()
+          (ensures eq (v_of s2) (concrete_merge (v_of lca) (v_of s1) (v_of s2))) = admit()
 
 let linearizable_s2_0' (lca s1 s2:st)
   : Lemma (requires consistent_branches lca s1 s2 /\
                     ops_of s2 = ops_of lca /\
                     merge_pre (v_of lca) (v_of s1) (v_of s2))
-          (ensures eq (v_of s1) (concrete_merge (v_of lca) (v_of s1) (v_of s2))) = ()
+          (ensures eq (v_of s1) (concrete_merge (v_of lca) (v_of s1) (v_of s2))) = admit()
+          
+#push-options "--z3rlimit 400" 
+let linearizable_gt0_s1' (lca s1 s2:st) (last1 last2:op_t)
+  : Lemma (requires do_pre (v_of s1) last1 /\ do_pre (v_of s2) last2 /\ 
+                    consistent_branches lca (do_st s1 last1) (do_st s2 last2) /\
+                    //consistent_branches lca s1 (do_st s2 last2) /\
+                    consistent_branches lca s1 s2 /\
+                    //is_prefix (ops_of lca) (ops_of s2) /\
+                    fst last1 <> fst last2 /\
+                    //First_then_second? (resolve_conflict last1 last2) /\
+                    //Remove? (snd last1) /\ Remove? (snd last2) /\ //all done
+                    //Add_after? (snd last1) /\ Remove? (snd last2) /\
+                    Add_after? (snd last1) /\ Add_after? (snd last2) /\ get_after_id last1 <> get_after_id last2 /\
+                    //Add_after? (snd last1) /\ Add_after? (snd last2) /\ get_after_id last1 = get_after_id last2 /\ fst last1 > fst last2 /\
+                    merge_pre (v_of lca) (do (v_of s1) last1) (do (v_of s2) last2) /\
+                    merge_pre (v_of lca) (v_of s1) (do (v_of s2) last2))
+                    //do_pre (concrete_merge (v_of lca) (v_of s1) (do (v_of s2) last2)) last1)
+                    
+          (ensures //merge_pre (v_of lca) (v_of s1) (do (v_of s2) last2) /\
+                   do_pre (concrete_merge (v_of lca) (v_of s1) (do (v_of s2) last2)) last1 (*/\                   
+                   eq (do (concrete_merge (v_of lca) (v_of s1) (do (v_of s2) last2)) last1)
+                      (concrete_merge (v_of lca) (do (v_of s1) last1) (do (v_of s2) last2)*)) =
+  assume ((Remove? (snd last2) /\ Add_after? (snd last1) ==> fst last1 <> get_rem_id last2) /\
+          (Add_after? (snd last1) /\ Add_after? (snd last2) ==>
+                      fst last1 <> get_after_id last2 /\ fst last2 <> get_after_id last1));
+  ()
 
 let rec lem_foldl (s:concrete_st) (l:log)
   : Lemma (requires do_pre_prop s l)
@@ -190,9 +216,11 @@ let linearizable_gt0_s1' (lca s1 s2:st) (last1 last2:op_t)
                     merge_pre (v_of lca) (do (v_of s1) last1) (do (v_of s2) last2))
           (ensures merge_pre (v_of lca) (v_of s1) (do (v_of s2) last2) /\
                    do_pre (concrete_merge (v_of lca) (v_of s1) (do (v_of s2) last2)) last1 /\
+                   
                    eq (do (concrete_merge (v_of lca) (v_of s1) (do (v_of s2) last2)) last1)
                       (concrete_merge (v_of lca) (do (v_of s1) last1) (do (v_of s2) last2))) = 
-  resolve_conflict_prop last1 last2;
+  
+  //resolve_conflict_prop last1 last2;
   merge_pre_prop lca s1 s2 last1 last2;
   lem_cond lca s1 s2 last1 last2
 
@@ -205,11 +233,12 @@ let linearizable_gt0_s2' (lca s1 s2:st) (last1 last2:op_t)
                     fst last1 <> fst last2 /\
                     Second_then_first? (resolve_conflict last1 last2) /\
                     merge_pre (v_of lca) (do (v_of s1) last1) (do (v_of s2) last2)) 
+          
           (ensures merge_pre (v_of lca) (do (v_of s1) last1) (v_of s2) /\
                    do_pre (concrete_merge (v_of lca) (do (v_of s1) last1) (v_of s2)) last2 /\
                    eq (do (concrete_merge (v_of lca) (do (v_of s1) last1) (v_of s2)) last2)
                       (concrete_merge (v_of lca) (do (v_of s1) last1) (do (v_of s2) last2))) = 
-  resolve_conflict_prop last1 last2;
+  //resolve_conflict_prop last1 last2;
   merge_pre_prop lca s1 s2 last1 last2;
   lem_cond lca s1 s2 last1 last2
 
@@ -235,7 +264,197 @@ let pre1_pre2_s1 (lca s1 s2:st)
   lem_inverse (ops_of lca) (ops_of s1);
   lastop_diff (ops_of lca) (ops_of s1);
   inverse_diff_id_s1' (ops_of lca) (ops_of s1) (ops_of s2)
-  
+
+#push-options "--z3rlimit 200" 
+(*let rec invalid_exec1 (lca s1 s2:st) (last2:op_t)
+  : Lemma (requires do_pre (v_of s2) last2 /\ 
+                    is_prefix (ops_of lca) (ops_of s1) /\ is_prefix (ops_of lca) (ops_of s2) /\
+                    distinct_ops (snoc (ops_of s2) last2) /\
+                    Remove? (snd last2))
+          (ensures (length (ops_of s1) > length (ops_of lca) ==> 
+                    (let _, last1 = un_snoc (ops_of s1) in
+                      (Add_after? (snd last1) ==>
+                           fst last1 <> get_rem_id last2))))
+          (decreases %[length (ops_of s1); length (ops_of s2)]) =
+  if ops_of lca = ops_of s1 then admit() //done
+  else 
+    (let s1' = inverse_st s1 in
+     let pre1, last1 = un_snoc (ops_of s1) in
+     lem_apply_log init_st (ops_of s1);
+     inverse_helper init_st pre1 last1;
+     if ops_of lca = pre1 then 
+       (if ops_of lca = ops_of s2 then admit() ///done
+        else 
+          (let s2' = inverse_st s2 in
+          let pre2, lastop2 = un_snoc (ops_of s2) in
+          do_prop (v_of s2') last2; 
+          lem_apply_log init_st (ops_of s2);
+          inverse_helper init_st pre2 lastop2;
+          //assert (mem_id_s (get_rem_id last2) (fst (v_of s2')) <==> do_pre (v_of s2') last2);
+          //pre1_pre2_s2 lca s1 s2;
+          if mem_id_s (get_rem_id last2) (fst (v_of s2')) then  //done
+            (admit();assume (do_pre (v_of s2') last2);
+             //assume (consistent_branches lca s1 (do_st s2' last2)); //can be done
+             invalid_exec1 lca s1 s2' last2)
+          else 
+            (assert (not (mem_id_s (get_rem_id last2) (fst (v_of s2'))));
+             if Add_after? (snd lastop2) && fst lastop2 = get_rem_id last2 then 
+              (lem_diff (snoc (ops_of s2) last2) (ops_of lca);
+               lem_diff (ops_of s2) (ops_of lca); 
+                //assert (mem_id (fst lastop2) (diff (ops_of s2) (ops_of lca)));
+                //assert (not (mem_id (fst lastop2) (ops_of lca)));
+                //assert (mem_id (fst lastop2) (ops_of s2));
+                lemma_append_count_assoc_fst (ops_of s2) (create 1 last2);
+                //assert (mem_id (fst lastop2) (snoc (ops_of s2) last2)); 
+                //assert (mem_id (fst lastop2) (diff (snoc (ops_of s2) last2) (ops_of lca)));
+                lem_diff (snoc (ops_of s1) last1) (ops_of lca);
+                //assert (mem_id (fst last1) (diff (snoc (ops_of s1) last1) (ops_of lca)));
+                admit()) 
+            else 
+              (assert (do_pre (v_of s2') last2);
+               assume (consistent_branches lca s1 (do_st s2' last2)); //can be done
+               invalid_exec1 lca s1 s2' last2))))
+     else admit())*)
+
+
+let rec invalid_exec1 (lca s1 s2:st) (last2:op_t)
+  : Lemma (requires do_pre (v_of s2) last2 /\ 
+                    consistent_branches lca s1 (do_st s2 last2) /\
+                    consistent_branches lca s1 s2 /\
+                    Remove? (snd last2))
+          (ensures (length (ops_of s1) > length (ops_of lca) ==> 
+                    (let _, last1 = un_snoc (ops_of s1) in
+                      (Add_after? (snd last1) ==>
+                           fst last1 <> get_rem_id last2))))
+          (decreases %[length (ops_of s1); length (ops_of s2)]) =
+  if ops_of lca = ops_of s1 then () //done
+  else 
+    (let s1' = inverse_st s1 in
+     let pre1, last1 = un_snoc (ops_of s1) in
+     lem_apply_log init_st (ops_of s1);
+     inverse_helper init_st pre1 last1;
+     if ops_of lca = pre1 then 
+       (if ops_of lca = ops_of s2 then () ///done
+        else 
+          (let s2' = inverse_st s2 in
+          let pre2, lastop2 = un_snoc (ops_of s2) in
+          do_prop (v_of s2') last2; 
+          lem_apply_log init_st (ops_of s2);
+          inverse_helper init_st pre2 lastop2;
+          //assert (mem_id_s (get_rem_id last2) (fst (v_of s2')) <==> do_pre (v_of s2') last2);
+          pre1_pre2_s2 lca s1 s2;
+          if mem_id_s (get_rem_id last2) (fst (v_of s2')) then 
+            (assert(do_pre (v_of s2') last2);
+             assume (consistent_branches lca s1 (do_st s2' last2)); //can be done
+             invalid_exec1 lca s1 s2' last2)
+          else 
+            (assert (not (mem_id_s (get_rem_id last2) (fst (v_of s2'))));
+            if Add_after? (snd lastop2) && fst lastop2 = get_rem_id last2 then 
+              (lem_diff (snoc (ops_of s2) last2) (ops_of lca);
+                lem_diff (ops_of s2) (ops_of lca); 
+                assert (mem_id (fst lastop2) (diff (ops_of s2) (ops_of lca)));
+                assert (not (mem_id (fst lastop2) (ops_of lca)));
+                assert (mem_id (fst lastop2) (ops_of s2));
+                lemma_append_count_assoc_fst (ops_of s2) (create 1 last2);
+                assert (mem_id (fst lastop2) (snoc (ops_of s2) last2)); 
+                assert (mem_id (fst lastop2) (diff (snoc (ops_of s2) last2) (ops_of lca)));
+                lem_diff (snoc (ops_of s1) last1) (ops_of lca);
+                assert (mem_id (fst last1) (diff (snoc (ops_of s1) last1) (ops_of lca))); 
+                ()) 
+            else 
+              (assert (do_pre (v_of s2') last2);
+               assume (consistent_branches lca s1 (do_st s2' last2)); //can be done
+               invalid_exec1 lca s1 s2' last2))))
+     else 
+       (admit()(*;let s1'' = inverse_st s1' in
+        let pre1', last1' = un_snoc pre1 in
+        lem_apply_log init_st pre1;
+        inverse_helper init_st pre1' last1';
+        if Add_after? (snd last1) && Add_after? (snd last1') && fst last1' = get_after_id last1 then //done
+         (admit();assume (do_pre (v_of s1'') (fst last1, snd last1')); //done
+          assume (consistent_branches lca (do_st s1'' (fst last1, snd last1')) (do_st s2 last2) /\ //can be done
+                  consistent_branches lca (do_st s1'' (fst last1, snd last1')) s2); //can be done
+          invalid_exec1 lca (do_st s1'' (fst last1, snd last1')) s2 last2)
+        else if Add_after? (snd last1) && Add_after? (snd last1') && fst last1' <> get_after_id last1 then //done
+          (admit();assume (not (mem_id_s (fst last1) (fst (v_of s1'')))); //done
+           assume (do_pre (v_of s1'') last1); //done
+           assume (consistent_branches lca (do_st s1'' last1) (do_st s2 last2) /\ //can be done
+                   consistent_branches lca (do_st s1'' last1) s2); //can be done
+           invalid_exec1 lca (do_st s1'' last1) s2 last2)
+        else if Remove? (snd last1') && Add_after? (snd last1) && get_rem_id last1' <> fst last1 then //done
+          (admit();assume (do_pre (v_of s1'') last1); //done
+           assume (consistent_branches lca (do_st s1'' last1) (do_st s2 last2) /\ //can be done
+                   consistent_branches lca (do_st s1'' last1) s2); //can be done
+           invalid_exec1 lca (do_st s1'' last1) s2 last2)
+        else 
+          admit()*))) //done
+
+let rec invalid_exec2 (lca s1 s2:st) (last2:op_t)
+  : Lemma (requires do_pre (v_of s2) last2 /\ 
+                    consistent_branches lca s1 (do_st s2 last2) /\
+                    consistent_branches lca s1 s2 /\
+                    Add_after? (snd last2))
+          (ensures (length (ops_of s1) > length (ops_of lca) ==> 
+                    (let _, last1 = un_snoc (ops_of s1) in
+                      (Add_after? (snd last1) ==>
+                           fst last1 <> get_after_id last2))))
+          (decreases %[length (ops_of s1); length (ops_of s2)]) =
+  if ops_of lca = ops_of s1 then admit() //done
+  else 
+    (let s1' = inverse_st s1 in
+     let pre1, last1 = un_snoc (ops_of s1) in
+     lem_apply_log init_st (ops_of s1);
+     inverse_helper init_st pre1 last1;
+     if ops_of lca = pre1 then 
+       (if ops_of lca = ops_of s2 then admit() ///done
+        else 
+          (let s2' = inverse_st s2 in
+          let pre2, lastop2 = un_snoc (ops_of s2) in
+          do_prop (v_of s2') last2; 
+          lem_apply_log init_st (ops_of s2);
+          inverse_helper init_st pre2 lastop2;
+          //assert (mem_id_s (get_rem_id last2) (fst (v_of s2')) <==> do_pre (v_of s2') last2);
+          pre1_pre2_s2 lca s1 s2;
+          if Remove? (snd lastop2) then //done
+            (admit();assume (do_pre (v_of s2') last2); //done
+             assume (consistent_branches lca s1 (do_st s2' last2)); //can be done
+             invalid_exec2 lca s1 s2' last2)
+          else if Add_after? (snd lastop2) && fst lastop2 <> get_after_id last2 then //todo
+            (admit();assume (do_pre (v_of s2') last2); //done
+             assume (consistent_branches lca s1 (do_st s2' last2)); //can be done
+             invalid_exec2 lca s1 s2' last2)
+          else 
+            (assume (Add_after? (snd lastop2) && fst lastop2 = get_after_id last2); 
+            lem_diff (snoc (ops_of s2) last2) (ops_of lca);
+            lem_diff (ops_of s2) (ops_of lca); 
+            lemma_append_count_assoc_fst (ops_of s2) (create 1 last2);
+            assume (mem_id (fst lastop2) (diff (snoc (ops_of s2) last2) (ops_of lca))); 
+            assume (mem_id (fst last1) (diff (ops_of s1) (ops_of lca)));
+            ())))
+     else 
+       (let s1'' = inverse_st s1' in
+        let pre1', last1' = un_snoc pre1 in
+        lem_apply_log init_st pre1;
+        inverse_helper init_st pre1' last1';
+        if Remove? (snd last1') then //done
+          (admit();assume (do_pre (v_of s1'') last1); //done
+           assume (consistent_branches lca (do_st s1'' last1) (do_st s2 last2) /\ //can be done
+                   consistent_branches lca (do_st s1'' last1) s2); //can be done
+           invalid_exec2 lca (do_st s1'' last1) s2 last2)
+        else if Add_after? (snd last1') && Add_after? (snd last1) && fst last1' <> get_after_id last1 then 
+          (admit();assume (do_pre (v_of s1'') last1); //done
+           assume (consistent_branches lca (do_st s1'' last1) (do_st s2 last2) /\ //can be done
+                   consistent_branches lca (do_st s1'' last1) s2); //can be done
+           invalid_exec2 lca (do_st s1'' last1) s2 last2)
+        else if Add_after? (snd last1') && Add_after? (snd last1) && fst last1' = get_after_id last1 then //done
+          (admit();assume (do_pre (v_of s1'') (fst last1, snd last1')); //done
+           assume (consistent_branches lca (do_st s1'' (fst last1, snd last1')) (do_st s2 last2) /\ //can be done
+                   consistent_branches lca (do_st s1'' (fst last1, snd last1')) s2); //can be done
+           invalid_exec2 lca (do_st s1'' (fst last1, snd last1')) s2 last2)
+        else admit())) //done
+
+          
+
 #push-options "--z3rlimit 400" 
 let rec invalid_exec1 (lca s1 s2:st) (last1 last2:op_t)
   : Lemma (requires do_pre (v_of s1) last1 /\ do_pre (v_of s2) last2 /\ 
@@ -246,9 +465,9 @@ let rec invalid_exec1 (lca s1 s2:st) (last1 last2:op_t)
           (ensures (fst last1 <> get_rem_id last2))
           (decreases %[length (ops_of s1); length (ops_of s2)]) = 
   if ops_of lca = ops_of s1 then
-    (if ops_of lca = ops_of s2 then ()
+    (if ops_of lca = ops_of s2 then admit()
      else 
-       (let s2' = inverse_st s2 in
+       (admit();let s2' = inverse_st s2 in
         let pre2, lastop2 = un_snoc (ops_of s2) in
         do_prop (v_of s2') last2; 
         lem_apply_log init_st (ops_of s2);
@@ -287,17 +506,17 @@ let rec invalid_exec1 (lca s1 s2:st) (last1 last2:op_t)
      pre1_pre2_s1 lca s1 s2;
      assume (fst lastop1 <> fst last1); //can be done
      if Add_after? (snd lastop1) && fst lastop1 <> get_after_id last1 then 
-       (assert (not (mem_id_s (fst last1) (fst (v_of s1'))));
+       (admit();assert (not (mem_id_s (fst last1) (fst (v_of s1'))));
         assert (do_pre (v_of s1') last1);
         assume (consistent_branches lca (do_st s1' last1) (do_st s2 last2)); //can be done
         invalid_exec1 lca s1' s2 last1 last2)
-     else if Add_after? (snd lastop1) && fst lastop1 = get_after_id last1 then  //check this case with full do_pre for add
+     else if Add_after? (snd lastop1) && fst lastop1 = get_after_id last1 then  //todo
        admit()
      else if Remove? (snd lastop1) && get_rem_id lastop1 <> fst last1 then
-       (assert (do_pre (v_of s1') last1); 
+       (admit();assert (do_pre (v_of s1') last1); 
         assume (consistent_branches lca (do_st s1' last1) (do_st s2 last2)); //can be done
         invalid_exec1 lca s1' s2 last1 last2)
-     else ()) //Remove? (snd lastop1) && get_rem_id lastop1 = fst last1
+     else admit()) //Remove? (snd lastop1) && get_rem_id lastop1 = fst last1
 
 
 let rec invalid_exec2 (lca s1 s2:st) (last1 last2:op_t)
@@ -305,10 +524,7 @@ let rec invalid_exec2 (lca s1 s2:st) (last1 last2:op_t)
                     consistent_branches lca (do_st s1 last1) (do_st s2 last2) /\
                     consistent_branches lca s1 s2 /\
                     Add_after? (snd last1) /\ Add_after? (snd last2) /\
-                    fst last1 <> fst last2 /\
-                    merge_pre (v_of lca) (do (v_of s1) last1) (do (v_of s2) last2) /\
-                    merge_pre (v_of lca) (v_of s1) (do (v_of s2) last2) /\
-                    merge_pre (v_of lca) (do (v_of s1) last1) (v_of s2))
+                    fst last1 <> fst last2)
           (ensures fst last1 <> get_after_id last2 (* /\ fst last2 <> get_after_id last1*))
           (decreases %[length (ops_of s1); length (ops_of s2)]) = 
   if ops_of lca = ops_of s1 then
